OneRuleAtATime.v
@@ -1,0 +1,609 @@
+Require Import SGA.Common SGA.Syntax SGA.Semantics.
+
+Require Import List.
+Import ListNotations.
+
+Open Scope bool_scope.
+
+Definition rule_ind' {TVar TFn : Type} (P : rule TVar TFn -> Prop)
+           (f : forall (var : TVar) (expr : rule TVar TFn),
+               P expr -> forall body : rule TVar TFn, P body -> P (Bind var expr body))
+           (f0 : forall var : TVar, P (Var var)) (f1 : P Skip) (f2 : forall cst : bits, P (Const cst))
+           (f3 : forall cond : rule TVar TFn,
+               P cond ->
+               forall tbranch : rule TVar TFn,
+                 P tbranch -> forall fbranch : rule TVar TFn, P fbranch -> P (If cond tbranch fbranch))
+           (f4 : P Fail) (f5 : forall (level : Level) (idx : nat), P (Read level idx))
+           (f6 : forall (level : Level) (idx : nat) (value : rule TVar TFn), P value -> P (Write level idx value))
+           (f7: forall (fn : TFn) (args : list (rule TVar TFn)),
+               List.Forall P args ->
+               P (Call fn args)) : forall r, P r.
+  refine (fix F (r : rule TVar TFn) : P r :=
+    match r as r0 return (P r0) with
+    | Bind var expr body => f var expr (F expr) body (F body)
+    | Var var => f0 var
+    | Skip => f1
+    | Const cst => f2 cst
+    | If cond tbranch fbranch => f3 cond (F cond) tbranch (F tbranch) fbranch (F fbranch)
+    | Fail => f4
+    | Read level idx => f5 level idx
+    | Write level idx value => f6 level idx value (F value)
+    | Call fn args => f7 fn args _
+    end).
+  revert args.
+  fix fargs 1.
+  destruct args; cbn; econstructor; eauto.
+Defined.
+
+Section EnvUpdates.
+  Context {RegEnv: Env nat bits}.
+
+  Definition commit_update V0 log : RegEnv.(env_t) :=
+    List.fold_right (fun entry V => match entry with
+                                  | LE LogWrite _ r bs => putenv V r bs
+                                  | _ => V
+                                  end)
+                    V0 log.
+
+  Lemma commit_update_assoc:
+    forall (V : RegEnv.(env_t)) (l l' : Log),
+      commit_update (commit_update V l) l' = commit_update V (l' ++ l).
+  Proof.
+    unfold commit_update; intros; rewrite fold_right_app; reflexivity.
+  Qed.
+
+  Section Semantics'.
+    Context {TVar: Type}.
+    Context {TFn: Type}.
+
+    Context {SigmaEnv: Env TFn ExternalFunction}.
+    Context {GammaEnv: Env TVar value}.
+
+    Fixpoint interp_scheduler
+          (V: RegEnv.(env_t))
+          (Sigma: SigmaEnv.(env_t))
+          (sched_log: Log)
+          (s: scheduler TVar TFn)
+          {struct s} :=
+    match s with
+    | Done => Some ([], sched_log)
+    | Try r s1 s2 =>
+      match interp_rule V Sigma env_nil sched_log [] r with
+      | Success (l, _) => match interp_scheduler V Sigma (l ++ sched_log) s1 with
+                         | Some (rs, log) => Some (r :: rs, log)
+                         | None => None
+                         end
+      | CannotRun => interp_scheduler V Sigma sched_log s2
+      | Stuck => None
+      end
+    end.
+
+    Definition interp_scheduler_and_update
+          (V: RegEnv.(env_t))
+          (Sigma: SigmaEnv.(env_t))
+          (s: scheduler TVar TFn)
+          l :=
+      match interp_scheduler V Sigma l s with
+      | Some (rs, log) => Some (rs, commit_update V log)
+      | None => None
+      end.
+
+    Definition update_one Sigma V r :=
+      match V with
+      | None => None
+      | Some V => match interp_scheduler_and_update V Sigma (Try r Done Done) [] with
+                 | Some (_, V') => Some V'
+                 | None => None
+                 end
+      end.
+
+    Definition latest_write l idx :=
+      log_find l idx (fun kind _ _ => match kind with
+                                   | LogWrite => true
+                                   | _ => false
+                                   end).
+
+    Lemma getenv_commit_update :
+      forall sl V idx val,
+        getenv V idx = Some val ->
+        getenv (commit_update V sl) idx =
+        match latest_write sl idx with
+        | Some {| val := val' |} => Some val'
+        | None => Some val
+        end.
+    Proof.
+      induction sl; cbn; intros.
+      - assumption.
+      - destruct a, kind, PeanoNat.Nat.eq_dec; subst;
+          try (erewrite IHsl by eassumption;
+               reflexivity).
+        + rewrite get_put_eq; reflexivity.
+        + rewrite get_put_neq by eauto.
+          erewrite IHsl by eassumption.
+          reflexivity.
+    Qed.
+
+    Lemma bool_result_Success :
+      forall b u,
+        bool_result b = Success u ->
+        b = true.
+    Proof.
+      destruct b; cbn; congruence.
+    Qed.
+
+    Require Import Ring_theory Ring Coq.setoid_ring.Ring.
+
+    Lemma log_forallb_app:
+      forall l l' reg (f: LogEntryKind -> Level -> bits -> bool),
+        log_forallb (l ++ l') reg f =
+        log_forallb l reg f && log_forallb l' reg f.
+    Proof.
+      unfold log_forallb.
+      intros; rewrite !forallb_app; reflexivity.
+    Qed.
+
+    Ltac set_forallb_fns :=
+      repeat match goal with
+             | [  |- context[log_forallb _ _ ?fn] ] =>
+               match fn with
+               | (fun _ => _) => set fn
+               end
+             end.
+
+    Lemma may_read0_app_sl :
+      forall sl sl' l idx,
+        may_read0 (sl ++ sl') l idx =
+        may_read0 sl l idx && may_read0 sl' l idx.
+    Proof.
+      unfold may_read0; intros.
+      rewrite !log_forallb_app.
+      ring_simplify.
+      f_equal.
+      f_equal.
+      rewrite <- !Bool.andb_assoc.
+      rewrite Bool.andb_diag; reflexivity.
+    Qed.
+
+    Lemma may_read1_app :
+      forall sl sl' idx,
+        may_read1 (sl ++ sl') idx =
+        may_read1 sl idx && may_read1 sl' idx.
+    Proof.
+      unfold may_read1; intros.
+      rewrite !log_forallb_app.
+      reflexivity.
+    Qed.
+
+    Lemma may_write_app_sl :
+      forall sl sl' l lvl idx,
+        may_write (sl ++ sl') l lvl idx =
+        may_write sl l lvl idx && may_write sl' l lvl idx.
+    Proof.
+      unfold may_write; intros.
+      destruct lvl; rewrite !log_forallb_app;
+        ring_simplify;
+        rewrite Bool.andb_diag;
+        reflexivity.
+    Qed.
+
+    Lemma log_find_in:
+      forall l idx P e,
+        log_find l idx P = Some e ->
+        List.In e l /\ e.(reg) = idx /\ P e.(kind) e.(level) e.(val) = true.
+    Proof.
+      unfold log_find; intros * H; destruct e; apply find_some in H.
+      destruct (PeanoNat.Nat.eq_dec idx reg); subst; cbn in *.
+      - intuition eauto.
+      - intuition discriminate.
+    Qed.
+
+    Ltac bool_step :=
+      match goal with
+      | [ H: _ && _ = true |- _ ] =>
+        apply andb_prop in H
+      | [ H: forallb _ (_ ++ _) = _ |- _ ] =>
+        rewrite forallb_app in H
+      | [ H: log_forallb (_ ++ _) _ _ = _ |- _ ] =>
+        rewrite log_forallb_app in H
+      | [ H: Some _ = Some _ |- _ ] =>
+        inversion H; subst; clear H
+      end.
+
+    Ltac cleanup_step :=
+      match goal with
+      | _ => discriminate
+      | _ => progress (subst; cbn)
+      | [ H: Some _ = Some _ |- _ ] =>
+        inversion H; subst; clear H
+      | [ H: (_, _) = (_, _) |- _ ] =>
+        inversion H; subst; clear H
+      | [ H: _ /\ _ |- _ ] =>
+        destruct H
+      end.
+
+    Lemma find_none_notb {A}:
+      forall (P: A -> bool) l,
+        (forall a, List.In a l -> P a = false) ->
+        find P l = None.
+    Proof.
+      induction l; cbn; intros * Hnot.
+      - reflexivity.
+      - pose proof (Hnot a).
+        destruct (P a); firstorder discriminate.
+    Qed.
+
+    Lemma may_read0_no_writes :
+      forall sl l idx,
+        may_read0 sl l idx = true ->
+        latest_write sl idx = None.
+    Proof.
+      unfold may_read0; intros.
+      repeat (cleanup_step || bool_step).
+      unfold log_forallb in *.
+      rewrite forallb_forall in *.
+      unfold latest_write, log_find.
+      apply find_none_notb.
+      intros a HIn.
+      repeat match goal with
+             | [ H: forall (_: LogEntry), _ |- _ ] => specialize (H a HIn)
+             end.
+      destruct a; cbn in *; destruct PeanoNat.Nat.eq_dec, kind; subst; try reflexivity.
+      destruct level; discriminate.
+    Qed.
+
+    Lemma find_app {A} :
+      forall sl sl' (P: A -> bool),
+        find P (sl ++ sl') =
+        match find P sl with
+        | Some e => Some e
+        | None => find P sl'
+        end.
+    Proof.
+      induction sl; cbn; intros.
+      - reflexivity.
+      - destruct (P a); try rewrite IHsl; reflexivity.
+    Qed.
+
+    Lemma log_find_app :
+      forall sl sl' idx P,
+        log_find (sl ++ sl') idx P =
+        match log_find sl idx P with
+        | Some e => Some e
+        | None => log_find sl' idx P
+        end.
+    Proof.
+      unfold log_find; eauto using find_app.
+    Qed.
+
+    Lemma latest_write0_app :
+      forall sl sl' idx,
+        latest_write0 (sl ++ sl') idx =
+        match latest_write0 sl idx with
+        | Some e => Some e
+        | None => latest_write0 sl' idx
+        end.
+    Proof.
+      unfold latest_write0; eauto using log_find_app.
+    Qed.
+
+    Lemma assert_size_success :
+      forall v n v',
+        assert_size v n = Success v' ->
+        v = v' /\ length v' = n.
+    Proof.
+      unfold assert_size; intros; destruct PeanoNat.Nat.eq_dec;
+        firstorder (congruence || discriminate).
+    Qed.
+
+    Lemma assert_size_eq :
+      forall a n,
+        length a = n ->
+        assert_size a n = Success a.
+    Proof.
+      unfold assert_size; intros; destruct PeanoNat.Nat.eq_dec; firstorder.
+    Qed.
+
+    Lemma may_read1_latest_write_is_0 :
+      forall l idx,
+        may_read1 l idx = true ->
+        latest_write l idx = latest_write0 l idx.
+    Proof.
+      induction l.
+      - reflexivity.
+      - intros * H.
+        simpl in H.
+        repeat (bool_step || cleanup_step).
+        destruct a; cbn; destruct PeanoNat.Nat.eq_dec, kind; cbn;
+          try apply (IHl _ ltac:(eassumption)).
+        destruct level; cbn in *; try discriminate; reflexivity.
+    Qed.
+
+    Lemma fold_left2_result_failure {A B B': Type} (f: A -> B -> B' -> result A) :
+      forall (l: list B) (l': list B') (a0: result A),
+        a0 = CannotRun \/ a0 = Stuck ->
+        fold_left2 (fun acc b b' =>
+                      result_bind acc (fun acc =>
+                      f acc b b')) l l' a0 = a0.
+    Proof.
+      induction l; destruct 1; destruct l'; subst; cbn in *; eauto.
+    Qed.
+
+    Require Import TypeSafety.
+
+    Lemma log_write_consistent_latest_write :
+      forall l (v: Typechecking.fenv nat nat) idx e n,
+        log_write_consistent l v ->
+        Typechecking.fn v idx n ->
+        latest_write l idx = Some e ->
+        length (e.(val)) = n.
+    Proof.
+      intros * Hcst Hin Hwrt.
+      pose proof (log_find_in _ _ _ _ Hwrt); cbn in *.
+      repeat cleanup_step; destruct e, kind; cbn in *; try discriminate.
+      eauto using eq_sym.
+    Qed.
+
+    Ltac t_step :=
+      match goal with
+      | _ => cleanup_step
+      | [ H: context[may_read0 (_ ++ _) _ _] |- _ ] =>
+        rewrite may_read0_app_sl in H
+      | [ H: context[may_read1 (_ ++ _) _] |- _ ] =>
+        rewrite may_read1_app in H
+      | [ H: context[may_write (_ ++ _) _ _ _] |- _ ] =>
+        rewrite may_write_app_sl in H
+      | [ H: Success _ = Success _ |- _ ] =>
+        inversion H; subst; clear H
+      | [ H: bool_result _ = Success _ |- _ ] =>
+        apply bool_result_Success in H
+      | [ H: opt_result Stuck ?x = Success _ |- _ ] =>
+        destruct x eqn:?; subst; cbn in H; try discriminate
+      | [ H: result_bind ?x _ = Success _ |- _ ] =>
+        destruct x eqn:?; cbn in H; try discriminate
+      | [ H: result_map ?x _ = Success _ |- _ ] =>
+        destruct x eqn:?; cbn in H; try discriminate
+      | [ H: match ?x with _ => _ end = Success _ |- _ ] =>
+        destruct x eqn:?; subst; cbn in H; try discriminate
+      | [ H: assert_size _ _ = Success _ |- _ ] =>
+        apply assert_size_Success in H
+      | [ H: env_equiv (Env := ?Env) ?f ?tenv ?env,
+             H': getenv ?env ?k = Some ?v |- _ ] =>
+        pose_once (and_fst H k v) H'
+      | [ H: env_equiv ?f ?tenv ?env,
+             H': getenv ?env ?k = None |- _ ] =>
+        pose_once (and_snd H k) H'
+      | _ =>
+        bool_step
+      | [ H: match ?x with _ => _ end = ?c |- _ ] =>
+        let c_hd := constr_hd c in
+        is_constructor c_hd; destruct x eqn:?
+      | _ => progress (unfold assert_bits in *)
+      end.
+
+    Ltac t :=
+      repeat t_step.
+
+    Lemma interp_rule_Success_call_consistent:
+      forall (args : list (rule TVar TFn)) (V : env_t RegEnv) (v : Typechecking.fenv nat nat)
+        (Sigma : env_t SigmaEnv) (Gamma : env_t GammaEnv) (sched_log rule_log l : Log) argvs,
+        env_equiv (length (A:=bool)) v V ->
+        log_write_consistent rule_log v ->
+        Forall
+          (fun r : rule TVar TFn =>
+             forall (V : env_t RegEnv) (v : Typechecking.fenv nat nat) (Sigma : env_t SigmaEnv)
+               (Gamma : env_t GammaEnv) (sl rule_log l : Log) (val : value),
+               env_equiv (length (A:=bool)) v V ->
+               log_write_consistent rule_log v ->
+               interp_rule V Sigma Gamma sl rule_log r = Success (l, val) -> log_write_consistent l v) args ->
+        forall (l1 : list bits) (argSizes : list nat),
+          length args = length argSizes ->
+          fold_left2_result
+            (fun '(rule_log, argvs) arg size =>
+            result_bind (interp_rule V Sigma Gamma sched_log rule_log arg) (fun '(rule_log, argv) =>
+            result_map (assert_bits argv size) (fun bs =>
+            (rule_log, bs :: argvs)))) args argSizes (rule_log, argvs) =
+          Success (l, l1) -> log_write_consistent l v.
+    Proof.
+      induction args; destruct argSizes; cbn in *; inversion 1; intros.
+      - t; eassumption.
+      - destruct interp_rule as [(?&[ | ?]) | | ] eqn:?; cbn in *.
+        + rewrite fold_left2_result_failure in H3; eauto || discriminate.
+        + unfold assert_size in *.
+          destruct PeanoNat.Nat.eq_dec; cbn in *.
+          * inversion H1; subst.
+            eapply (IHargs V v Sigma Gamma sched_log l0); eauto.
+          * rewrite fold_left2_result_failure in H3; eauto || discriminate.
+        + rewrite fold_left2_result_failure in H3; eauto || discriminate.
+        + rewrite fold_left2_result_failure in H3; eauto || discriminate.
+    Qed.
+
+    Lemma interp_rule_Success_consistent:
+      forall r {V v Sigma Gamma} sl rule_log l val,
+        env_equiv (@length bool) v V ->
+        log_write_consistent rule_log v ->
+        interp_rule V Sigma Gamma sl rule_log r = Success (l, val) ->
+        log_write_consistent l v.
+      induction r using rule_ind'; cbn; intros; try solve [t; eauto with types].
+      - t.
+        destruct a, sig; cbn in *.
+        eapply interp_rule_Success_call_consistent; eauto.
+    Qed.
+
+    Lemma interp_rule_commit_call:
+      forall args : list (rule TVar TFn),
+        Forall
+          (fun r : rule TVar TFn =>
+             forall (V : env_t RegEnv) (v : Typechecking.fenv nat nat) (Sigma : env_t SigmaEnv)
+               (Gamma : env_t GammaEnv) (sl sl' rule_log l : Log) (val : value),
+               env_equiv (length (A:=bool)) v V ->
+               log_write_consistent sl v ->
+               log_write_consistent sl' v ->
+               interp_rule V Sigma Gamma (sl ++ sl') rule_log r = Success (l, val) ->
+               interp_rule (commit_update V sl') Sigma Gamma sl rule_log r = Success (l, val)) args ->
+        forall (V : env_t RegEnv) (Sigma : env_t SigmaEnv) (Gamma : env_t GammaEnv) (sl sl' rule_log l : Log)
+               (argSizes : list nat) v argvs,
+          length args = length argSizes ->
+          env_equiv (length (A:=bool)) v V ->
+          log_write_consistent sl v ->
+          log_write_consistent sl' v ->
+          forall l1 : list bits,
+            fold_left2_result
+              (fun '(rule_log, argvs) arg size =>
+                  result_bind (interp_rule V Sigma Gamma (sl ++ sl') rule_log arg) (fun '(rule_log, argv) =>
+                  result_map (assert_bits argv size) (fun bs =>
+                  (rule_log, bs :: argvs)))) args argSizes (rule_log, argvs) =
+            Success (l, l1) ->
+            fold_left2_result
+              (fun '(rule_log, argvs) arg size =>
+                  result_bind (interp_rule (commit_update V sl') Sigma Gamma sl rule_log arg) (fun '(rule_log, argv) =>
+                  result_map (assert_bits argv size) (fun bs =>
+                  (rule_log, bs :: argvs)))) args argSizes (rule_log, argvs) =
+            Success (l, l1).
+    Proof.
+      induction args; destruct argSizes; cbn in *; inversion 1; intros.
+      - t. reflexivity.
+      - destruct (interp_rule V Sigma Gamma (sl ++ sl') rule_log a) as [(? & ?) | | ] eqn:?; cbn in *.
+        + inversion H; subst.
+          eapply H8 in Heqr; eauto using log_write_consistent_nil.
+          rewrite Heqr; cbn.
+          destruct assert_bits; cbn in *.
+          * move IHargs at bottom.
+            unfold fold_left2_result in *.
+            eapply IHargs; eauto.
+          * rewrite fold_left2_result_failure in H5; eauto || discriminate.
+          * rewrite fold_left2_result_failure in H5; eauto || discriminate.
+        + rewrite fold_left2_result_failure in H5; eauto || discriminate.
+        + rewrite fold_left2_result_failure in H5; eauto || discriminate.
+    Qed.
+
+    Lemma interp_rule_commit:
+      forall r {V v Sigma Gamma} sl sl' rule_log l val,
+        env_equiv (@length bool) v V ->
+        log_write_consistent sl v ->
+        log_write_consistent sl' v ->
+        interp_rule V Sigma Gamma (sl ++ sl') rule_log r = Success (l, val) ->
+        interp_rule (commit_update V sl') Sigma Gamma sl rule_log r = Success (l, val).
+    Proof.
+      induction r using rule_ind'; cbn; intros V v Sigma Gamma * Heqiv Hcst Hcst'; intros; try congruence.
+      - (* Bind *)
+        t. erewrite IHr1; cbn; eauto.
+      - (* If *)
+        t;
+          erewrite IHr1; cbn; eauto;
+            [ erewrite IHr2; cbn; eauto |
+              erewrite IHr3; cbn; eauto ].
+      - destruct level.
+        + (* Read0 *)
+          t.
+
+          erewrite getenv_commit_update by eassumption.
+          destruct latest_write eqn:?; cbn.
+          * destruct l; cbn.
+            rewrite H1; cbn.
+            erewrite may_read0_no_writes in Heqo0; eauto.
+            discriminate.
+
+          * rewrite H1; cbn.
+            reflexivity.
+
+        + (* Read1 *)
+          t;
+            rewrite app_assoc in Heqo0;
+            rewrite latest_write0_app in Heqo0;
+            t;
+            erewrite getenv_commit_update by eassumption.
+          destruct latest_write eqn:?; cbn.
+          * destruct l; cbn.
+            rewrite H2; cbn.
+
+            lazymatch goal with
+            | [ H: latest_write ?l ?idx = Some ?entry |- _ ] =>
+              let v0 := (eval cbn in entry.(Semantics.val)) in
+              change v0 with (entry.(Semantics.val));
+              erewrite log_write_consistent_latest_write
+            end; eauto.
+            rewrite assert_size_eq by auto; cbn.
+            reflexivity.
+          * rewrite H2; cbn.
+            rewrite assert_size_eq by auto; cbn.
+            reflexivity.
+          *
+
+            rewrite may_read1_latest_write_is_0 by eassumption.
+
+            rewrite Heqo0; cbn.
+            rewrite H2; cbn.
+            reflexivity.
+
+          * rewrite may_read1_latest_write_is_0 by eassumption.
+            rewrite Heqo0; cbn.
+            rewrite H1; cbn.
+            reflexivity.
+
+      - t.
+        erewrite getenv_commit_update by eassumption.
+        destruct latest_write eqn:?; cbn.
+        + destruct l; cbn.
+          erewrite IHr by eassumption; cbn.
+          rewrite H1; cbn.
+
+            lazymatch goal with
+            | [ H: latest_write ?l ?idx = Some ?entry |- _ ] =>
+              let v0 := (eval cbn in entry.(Semantics.val)) in
+              change v0 with (entry.(Semantics.val));
+              erewrite log_write_consistent_latest_write
+            end; eauto.
+            rewrite assert_size_eq by auto; cbn.
+
+          reflexivity.
+        + erewrite IHr by eassumption; cbn.
+          rewrite H1; cbn.
+          rewrite assert_size_eq by auto; cbn.
+          reflexivity.
+
+      - t.
+        destruct a, sig; cbn in *.
+        erewrite interp_rule_commit_call; cbn; eauto.
+    Qed.
+
+  Lemma OneRuleAtATime:
+    forall Sigma s V v rs V' l0,
+      env_equiv (@length bool) v V ->
+      log_write_consistent l0 v ->
+      interp_scheduler_and_update V Sigma s l0 = Some (rs, V') ->
+      List.fold_left (update_one Sigma) rs (Some (commit_update V l0)) = Some V'.
+  Proof.
+    induction s; cbn.
+    - inversion 3; subst; cbn in *; eauto.
+    - intros * Hequiv Hcst Heq.
+      unfold interp_scheduler_and_update in *; cbn in *.
+      destruct interp_rule as [(l & ?) | | ] eqn:?; try discriminate.
+
+      + destruct interp_scheduler as [(? & ?) | ] eqn:?; try discriminate;
+          inversion Heq; subst; clear Heq; cbn.
+        unfold interp_scheduler_and_update; cbn.
+        enough (interp_rule (commit_update V l0) Sigma env_nil [] [] r = Success (l, v0)) as H.
+        rewrite H.
+        rewrite commit_update_assoc.
+        rewrite app_nil_r.
+        eapply IHs1.
+        eassumption.
+        apply log_write_consistent_app.
+        eassumption.
+        eauto using interp_rule_Success_consistent, log_write_consistent_nil.
+        rewrite Heqo.
+        reflexivity.
+        eapply interp_rule_commit.
+        eassumption.
+        eapply log_write_consistent_nil.
+        eassumption.
+        rewrite app_nil_l.
+        assumption.
+      + eapply IHs2.
+        eassumption.
+        eassumption.
+        destruct interp_scheduler as [(? & ?) | ] eqn:?; try discriminate.
+        inversion Heq; subst.
+        reflexivity.
+  Qed.
+  End Semantics'.
